

1. (a) Find the general solution of

$$tx'(t) = x(t) + 3t^2$$

Solution: First, notice that,

$$tx'(t) = x(t) + 3t^2 \Rightarrow x'(t) - \frac{1}{t}x(t) = 3t.$$

This is a first order linear differential equation. Let

$$\mu(t) = e^{\int -\frac{1}{t} dt} = e^{-\ln t} = \frac{1}{t}$$

be the integrating factor. Then,

$$\begin{aligned} \frac{1}{t}x' - \frac{1}{t^2}x &= 3 \Rightarrow \int (tx)' dt = \int 3 dt \\ &\Rightarrow \frac{1}{t}x = 3t + C \\ &\Rightarrow \boxed{x(t) = 3t^2 + Ct} \end{aligned}$$

- (b) Find the flow transformation $\Phi_{t,t_0}(x)$ specified by this equation

Solution: Let us choose C such that $x(t_0) = x$,

$$x(t_0) = 3t_0^2 + Ct_0 \Rightarrow C = \frac{x - 3t_0^2}{t_0}.$$

Thus, our flow transformation will be

$$x(t) = \boxed{\Phi_{t,t_0}(x) = 3t^2 + \frac{x - 3t_0^2}{t_0}t}$$

- (c) Find the particular solution $x(t)$ that satisfies $x(1) = 2$

Solution:

$$\begin{aligned} x(t) &= 3t^2 + Ct \Rightarrow x(1) = 2 = 3(1)^2 + C(1) \\ &\Rightarrow C = -1 \\ &\Rightarrow \boxed{x(t) = 3t^2 - 1} \end{aligned}$$

2. (a) Find the general solution of

$$x'(t) + \frac{1}{3}x(t) = e^t x^4(t)$$

Solution: Start by dividing the entire equation by $x^4(t)$ to get

$$x^{-4}x' + \frac{1}{3}x^{-3} = e^t.$$

Now, this is clearly a Bernoulli differential equation, so consider the change of variable

$$v = x^{-3} \Rightarrow v' = -3x^{-4}x' \Rightarrow -\frac{1}{3}v' = x^{-4}x'.$$

Applying our change of variables we can see that

$$-\frac{1}{3}v' + \frac{1}{3}v = e^t \Rightarrow v' - v = -3e^t.$$

This is now a linear differential equation, so we will let our integrating factor be

$$\mu(t) = e^{\int -1 dt} = e^{-t}.$$

Multiplying through by the integrating factor and solving shows

$$\begin{aligned} e^{-t}v' - e^{-t}v &= -3 \Rightarrow \int (e^{-t}v)' dt = \int -3 dt \\ &\Rightarrow e^{-t}v = -3t + C \\ &\Rightarrow v = -3te^t + Ce^t \\ &\Rightarrow x^{-3} = -3te^t + Ce^t \\ &\Rightarrow \boxed{x(t) = (-3te^t + Ce^t)^{-1/3}} \end{aligned}$$

- (b) Find the particular solution $x(t)$ that satisfies $x(1) = 2$. Over what time interval $t \in (a, b)$ is the solution a continuously differentiable function?

Solution: First we will solve for C ,

$$\begin{aligned} x(1) = 2 &\Rightarrow 2 = (-3(1)e^1 + Ce^1)^{-1/3} \\ &\Rightarrow 2^{-3} = e(C - 3) \\ &\Rightarrow \frac{1}{8e} = C - 3 \\ &\Rightarrow \frac{1}{8e} + 3 = C \end{aligned}$$

Thus, our particular solution is

$$\boxed{x(t) = \left(-3te^t + \left(\frac{1}{8e} + 3 \right) e^t \right)^{-1/3} = \frac{1}{\sqrt[3]{e^t \left(3(1-t) + \frac{1}{8e} \right)}}$$

Since this is a rational function we must check when the denominator equals 0,

$$\begin{aligned} 3(1-t) + \frac{1}{8e} = 0 &\Rightarrow 3 + \frac{1}{8e} = 3t \\ &\Rightarrow t = 1 + \frac{1}{24e}. \end{aligned}$$

Note that we were able to drop e^t from the denominator since it will never be 0. Thus, since our interval must contain the initial condition,

$$x(t) \text{ is continuously differentiable for all } t \in \left(-\infty, 1 + \frac{1}{24e}\right).$$

3. (a) Find the general solution of

$$tx'(t) = tx^2(t) - x(t) - \frac{1}{t}$$

Solution: First, rewrite the equation as

$$x' = x^2 - \frac{1}{t}x - \frac{1}{t^2}.$$

This is a Riccati equation. Since all the coefficients are powers of t we will consider a particular solution in the form $x_1 = ct^\alpha$ for $c, \alpha \in \mathbb{R}$,

$$\alpha ct^{\alpha-1} = c^2 t^{2\alpha} - ct^{\alpha-1} - t^{-2}$$

Since all the powers of t must be equal we can solve for α :

$$\alpha - 1 = 2\alpha = -2 \Rightarrow \alpha = -1.$$

This allows us to cancel all the t 's from the equation leaving us with

$$\begin{aligned} c &= c^2 - c - 1 \Rightarrow c^2 - 1 = 0 \\ &\Rightarrow (c-1)(c+1) = 0 \\ &\Rightarrow c = -1, 1. \end{aligned}$$

Thus, we have $x_1 = t^{-1}$ or $x_1 = -t^{-1}$. Choosing $x_1 = t^{-1}$ we can solve for the general solution with the formula

$$x(t) = x_1(t) + u(t)$$

where $u(t)$ is a solution to the equation

$$u' = (q + 2rx_1)u + ru^2$$

for $q = -t^{-1}$ (coefficient of the linear term) and $r = 1$ (coefficient of the quadratic term). We

can solve this as follows:

$$\begin{aligned}
 u' &= (-t^{-1} + 2(1)t^{-1})u + u^2 \Rightarrow u'u^{-2} - t^{-1}u^{-1} = 1 \\
 &\Rightarrow \text{Let } v = u^{-1} \Rightarrow v' = -u^{-2}u' \\
 &\Rightarrow v' + t^{-1}v = -1 \\
 &\Rightarrow \mu(t) = e^{\int t^{-1} dt} = e^{\ln t} = t \\
 &\Rightarrow tv' + v = -t \\
 &\Rightarrow \int (tv)' dt = \int -t dt \\
 &\Rightarrow tv = -\frac{1}{2}t^2 + C \\
 &\Rightarrow v = -\frac{1}{2}t + \frac{C}{t} \\
 &\Rightarrow u^{-1} = -\frac{1}{2} + \frac{C}{t} \\
 &\Rightarrow u = \left(-\frac{1}{2}t + \frac{C}{t}\right)^{-1}.
 \end{aligned}$$

Thus, our general solution is

$$x(t) = x_1(t) + u(t) = \frac{1}{t} + \frac{1}{-\frac{1}{2}t + \frac{C}{t}} = \boxed{\frac{t^2 + C}{t(C - t^2)}}$$

- (b) For any (x_0, t_0) with $t_0 > 0$, find the solution $x(t)$ of this equation that satisfies $x(t_0) = x_0$

Solution: We can solve for C using the initial conditions as follows,

$$\begin{aligned}
 x(t_0) &= x_0 \Rightarrow x_0 = \frac{t_0^2 + C}{t_0(C - t_0^2)} \\
 &\Rightarrow x_0 t_0 (C - t_0^2) = t_0^2 + C \\
 &\Rightarrow C x_0 t_0 - x_0 t_0^3 = t_0^2 + C \\
 &\Rightarrow C(x_0 t_0 - 1) = t_0^2 + x_0 t_0^3 \\
 &\Rightarrow C = \frac{t_0^2 + x_0 t_0^3}{x_0 t_0 - 1}.
 \end{aligned}$$

Thus, our particular solution is

$$x(t) = \frac{t^2 + \frac{t_0^2 + x_0 t_0^3}{x_0 t_0 - 1}}{t \left(\frac{t_0^2 + x_0 t_0^3}{x_0 t_0 - 1} - t^2 \right)} = \boxed{\frac{x_0 t_0 (t^2 + t_0^2) - (t^2 - t_0^2)}{t[x_0 t_0 (t_0^2 - t^2) + (t^2 + t_0^2)]}}$$

- (c) Write down a formula for the flow transformation Φ_{t,t_0} generated by this equation. Verify explicitly that $\Phi_{3,2}(\Phi_{2,1}(x)) = \Phi_{3,1}(x)$ for all x

Solution: We choose C such that $x(t_0) = x$. By substituting x_0 for x in our work in part (b) we can see that

$$C = \frac{xt_0^3 + t_0^2}{xt_0 - 1} \Rightarrow x(t) = \frac{xt_0(t^2 + t_0^2) - (t^2 - t_0^2)}{t[xt_0(t_0^2 - t^2) + (t^2 + t_0^2)]}.$$

It follows that the flow transformation is

$$\Phi_{t_1,t_0}(x) = x(t_1) = \frac{xt_0(t_1^2 + t_0^2) - (t_1^2 - t_0^2)}{t_1[xt_0(t_0^2 - t_1^2) + (t_1^2 + t_0^2)]}$$

In order to verify that $\Phi_{3,2}(\Phi_{2,2}(x)) = \Phi_{3,1}(x)$ we will need the following:

$$\begin{aligned}\Phi_{2,1}(x) &= \frac{x(1+4) - (4-1)}{2(x(1-4) + (4+1))} = \frac{5x-3}{10-6x} \\ \Phi_{3,2}(x) &= \frac{x(2)(9+4) - (9-4)}{3(x(2)(4-9) + (9+4))} = \frac{26x-5}{39-30x} \\ \Phi_{3,1}(x) &= \frac{x(9+1) - (9-1)}{3(x(1-9) + (9+1))} = \frac{10x-8}{30-24x}.\end{aligned}$$

We can now verify that

$$\begin{aligned}\Phi_{3,2}(\Phi_{2,1}(x)) &= \frac{26\left(\frac{5x-3}{10-6x}\right) - 5}{39 - 30\left(\frac{5x-3}{10-6x}\right)} = \frac{26(5x-3) - 5(10-6x)}{39(10-6x) - 30(5x-3)} \\ &= \frac{130x - 78 - 50 + 30x}{390 - 234x - 150x + 90} \\ &= \frac{160x - 128}{480 - 384x} \\ &= \frac{10x - 8}{30 - 24x} = \Phi_{3,1}(x)\end{aligned}$$

4. Consider the equation

$$x'(t) = 2t \frac{t^2 + x(t)}{t^2 - x(t)} \tag{1}$$

with the change of variable

$$y(t) = \frac{x(t)}{t^2} \tag{2}$$

for $t > 0$.

- (a) Show that $x(t)$ solves (1) for $t > 0$ if, and only if, $y(t)$ solves a separable equation for $t > 0$.

Solution: We start by assuming that $x(t)$ solves (1) for $t > 0$ in order to show that $y(t)$ solves a separable equation for $t > 0$. If $x(t)$ solves (1) then,

$$y(t) = \frac{x(t)}{t^2} \Rightarrow x = t^2 y \Rightarrow x' = 2ty + t^2 y'.$$

Thus,

$$\begin{aligned}
 2t \left(\frac{t^2 + t^2 y}{t^2 - t^2 y} \right) &= 2ty + t^2 y' \\
 \Rightarrow 2t \left(\frac{1+y}{1-y} - y \right) &= t^2 y' \\
 \Rightarrow 2t \left(\frac{1+y^2}{1-y} \right) &= t^2 y' \\
 \Rightarrow \frac{2}{t} \left(\frac{1+y^2}{1-y} \right) &= \frac{dy}{dt} \\
 \Rightarrow \frac{2}{t} dt &= \frac{1-y}{1+y^2} dy. \tag{3}
 \end{aligned}$$

This is a seperable equation. We can prove that assuming $y(t)$ solves a seperable equation is a sufficient condition for $x(t)$ solving (1) by assuming that $y(t)$ solves (3) and following the steps above in reverse.

- (b) Find the solution of (2) with $y(1) = y_0, y_0 \neq 1$

Solution: Starting with (3) we have

$$\begin{aligned}
 \int \frac{2}{t} dt &= \int \frac{1-y}{1+y^2} dt = \int \frac{1}{1+y^2} - \frac{y}{1+y^2} dy \\
 \Rightarrow 2 \ln t + C &= \arctan(y) - \frac{1}{2} \ln(1+y^2).
 \end{aligned}$$

Applying the initial condition we can see that

$$y(1) = y_0 \Rightarrow C = \arctan(y_0) - \frac{1}{2} \ln(1+y_0^2).$$

Thus, the general solution is

$$2 \ln t + \arctan(y_0) - \frac{1}{2} \ln(1+y_0^2) = \arctan(y) - \frac{1}{2} \ln(1+y^2)$$

- (c) Find the solution of (1) with $x(1) = x_0, x_0 \neq 1$

Solution: We start by noticing that

$$x(t) = t^2 y(t) \Rightarrow x(1) = y(1) \Rightarrow x_0 = y_0.$$

Thus, the general solution for $x(t)$ is

$$2 \ln t + \arctan(x_0) - \frac{1}{2} \ln(1+x_0^2) = \arctan(t^{-2}x) - \frac{1}{2} \ln(1+t^{-4}x^2)$$

5. Find the general solution of the equation

$$tx''(t) = 1 + (x'(t))^2$$

Solution: Consider the change of variables $y = x'$ and substitute:

$$\begin{aligned} ty' &= 1 + y^2 \Rightarrow t \frac{dy}{dt} = 1 + y^2 \\ &\Rightarrow \int \frac{1}{1 + y^2} dy = \int \frac{1}{t} dt \\ &\Rightarrow \arctan(y) = \ln(t) + C \\ &\Rightarrow y = \tan(\ln(t) + C). \end{aligned}$$

It follows that

$$x(t) = \int y(t) dt = \boxed{\int \tan(\ln t + C) dt}$$

for $C \in \mathbb{R}$. Note that I was unable to figure out how to integrate the explicit function for y .

⁰L^AT_EX code for this document can be found on github [here](#)